%!TEX root = thesis.tex

\chapter{Derivations and Equations}
\label{app:Derivations}
% --------------------------------------------------------- %
\section{Belief Update}
\label{app:BeliefUpdates}
% --------------------------------------------------------- %
\begin{equation}
  B_t^i \defeq p(S_t = i | A_{1:t}, O_{1:t})
\end{equation}

\begin{subequations}\label{belief_update}
  \begin{align}
    b_t^j &= p(S_t = j | a_{1:t}, o_{1:t})\label{belief_state} \\
          &= \frac{ p(S_t = j, o_t | a_{1:t}, o_{1:t-1}) } { p(o_t) } \\
          &= \frac{ p(o_t | S_t = j, a_{1:t}, o_{1:t-1}) p(S_t = j | a_{1:t}, o_{1:t-1})} { p(o_t) } \\
          \intertext{and since $o_t$ is independent of $o_{1:t-1}$ we can write}
          &= \frac{ p(o_t | S_t = j, a_{1:t}) p(S_t = j | a_{1:t}, o_{1:t-1})} { p(o_t) } \\
          &= \frac{ p(o_t | S_t = j, a_{1:t}) \sum_{i} p(S_t = j, S_{t-1} = i | a_{1:t}, o_{1:t-1})} { p(o_t) } \\
          &= \frac{ p(o_t | S_t = j, a_{1:t}) \sum_{i} p(S_t = j | S_{t-1} = i, a_{1:t}, o_{1:t-1}) p(S_{t-1} = i | a_{1:t-1}, o_{1:t-1})} { p(o_t) } \\
          \intertext{Markovian assumption; given $S_{t-1}$, $S_t$ is independent of $a_{1:t-1}, o_{1:t-1}$ so we get}
          &= \frac{ p(o_t | S_t = j, a_{1:t}) \sum_{i} p(S_t = j | S_{t-1} = i, a_t) p(S_{t-1} = i | a_{1:t-1}, o_{1:t-1}) } { p(o_t) } \\
          \intertext{Using \eqref{belief_state} we can write}
          &= \frac{ p(o_t | S_t = j, a_{1:t}) \sum_{i} p(S_t = j | S_{t-1} = i, a_t) b_{t-1}^i } { p(o_t) } \\
          \intertext{Markovian assumption again; given $S_t$, $o_t$ is independent of $a_{1:t-1}$ so we get}
          &= \frac{ p(o_t | S_t = j, a_t) \sum_{i} p(S_t = j | S_{t-1} = i, a_t) b_{t-1}^i } { p(o_t) }
  \end{align}
\end{subequations}
If the state never changes we have
\begin{equation}\label{fixed_target}
  p(S_t = j | S_{t-1} = i, a_t) =
  \begin{cases}
    1 & \text{if $j = i$} \\
    0 & \text{otherwise}
  \end{cases}
\end{equation}
and then \eqref{belief_update} becomes
\begin{equation}\label{belief_update_fixed}
  b_t^j = \frac{ p(o_t | S_t = j, a_t) b_{t-1}^j }{ p(o_t) }
\end{equation}
where $p(o_t)$ can be treated as a normalization factor.

% --------------------------------------------------------- %
\section{Observations}
% --------------------------------------------------------- %
The observation model is
\begin{equation}\label{app:ObservationModel}
  \begin{split}
    O_t^j &= \delta (S_t, j) d_{j,k} + Z_t^j \\
          &= \begin{cases}
                d_{j,k} + Z_t^j & \text{if $S_t = j$}\\
                Z_t^j           & \text{otherwise}
             \end{cases}
  \end{split}
\end{equation}
where $Z_t^j$ is zero mean, unit variance Gaussian random noise (i.e. white noise) and in the case of an exponential-decay vision system 
\begin{equation}
  d_{j,k} = 3 \cdot e^{-dist(j,k)}
\end{equation}
where $dist(j,k)$ is the Euclidean distance between locations $j$ and $k$.

We assume that given an image, individual observations (i.e. each pixel)
\begin{equation}
  o_t = (o_t^1, \dotsc, o_t^{|\mathcal{S}|})
\end{equation}
are conditionally independent. Then we can write the probability of an observation as
\begin{subequations}
  \begin{align}
    p(o_t | S_t = i, A_t = k) 
      &= \prod_j p(o_t^j | S_t = i, A_t = k) \\
      &= p(o_t^i | S_t = i, A_t = k) \prod_{j \neq i} p(o_t^j | S_t = i, A_t = k) \\
      \intertext{Given the observation model from equation \eqref{app:ObservationModel} we get}
      &= \gaussianexp{o_t^i - d_{i,k}} \prod_{j \neq i} \gaussianexp{o_t^j} \\
      &= \frac{1}{\sqrt{2\pi}} \frac{\gaussianexppart{o_t^i - d_{i,k}}}{\gaussianexppart{o_t^i}} \prod_j \gaussianexp{o_t^j} \\
      &= \frac{\gaussianexppart{o_t^i - d_{i,k}}}{\gaussianexppart{o_t^i}} Z \\
      &= \exp((o_t^i - \frac{d_{i,k}}{2}) d_{i,k}) K
  \end{align}
\end{subequations}
where $K$ is a constant. Ignoring the constant $K$ and terms not containing $o_t^i$ we can write
\begin{equation}
  \label{app:ProportionalObservationLikelihood}
  p(o_t | S_t = i, A_t = k) \propto \exp{(d_{i,k} o_t^i)}
\end{equation}

% --------------------------------------------------------- %
\section{Proportional Belief Update}
% --------------------------------------------------------- %
Combining \eqref{belief_update_fixed} and \eqref{app:ProportionalObservationLikelihood} yields the proportional belief update
\begin{equation}
  % b_{t+1}^i \propto \exp(\alpha_{i,k} d_{i,k}) b_t^i
  b_{t+1}^i \propto \exp{(d_{i,k} o_t^i)} b_t^i
\end{equation}
